Ввёл кучу лемм, тригонометрию. Определил типы координат и их преобразования друг в друга.

Test_Float.fs
@@ -6,7 +6,6 @@ type float = System.Single
 
 let to_string (x: float) : string = x.ToString()
 
-let of_pair (mant: BigInteger, exp: BigInteger) : float = System.Single.Parse $"{mant}e{exp}"
 let to_pair (x: float) : BigInteger * BigInteger =
     Seq.initInfinite (fun exp ->
         let x' = x * single (pown 10 exp)
@@ -15,15 +14,30 @@ let to_pair (x: float) : BigInteger * BigInteger =
         if System.Single.IsInteger value
         then Some (BigInteger value, BigInteger -exp)
         else None)
+let of_pair (mant: BigInteger, exp: BigInteger) : float = System.Single.Parse $"{mant}e{exp}"
+let of_int (x: BigInteger) : float = single x
 
 let zero : float = 0f
-let one : float = -1f
+let one : float = 1f
 
 let add (a: float) (b: float) : float = a + b
 let sub (a: float) (b: float) : float = a - b
+let neg (a: float) : float = -a
 let mul (a: float) (b: float) : float = a * b
+let div (a: float) (b: float) : float = a / b
 
 let gt (a: float) (b: float) = a > b
 let lt (a: float) (b: float) = a < b
 let gte (a: float) (b: float) = a >= b
 let lte (a: float) (b: float) = a <= b
+
+let abs (a: float) : float = abs a
+
+let pi: float = System.Single.Pi
+let piHalf: float = System.Single.Pi / 2f
+
+let inline sin (x: float) : float = float.Sin(x / 180f * pi)
+let inline cos (x: float) : float = float.Cos(x / 180f * pi)
+let inline sinCos (x: float) : struct (float * float) = float.SinCos(x / 180f * pi)
+let inline arctg (x: float) (y: float) : float = float.Atan2(y, x) * 180f / pi
+let inline hypot (x: float) (y: float) : float = float.Hypot(x, y)
