Test.Float.fsti
@@ -18,18 +18,26 @@ type powerType = e: int{e <= 0}
 type mant_pow' = mantType & powerType
 type mant_pow = x: mant_pow'{x._1 % 10 = 0 ==> x._2 = 0}
 
-val of_pair (mant_power: mant_pow) : float
 val to_pair (x: float) : mant_pow
+val of_pair (mant_power: mant_pow) : float
+let of_int (x: int) : float = of_pair (x, 0)
 
 val lemma_of_to_inv (x: float) : Lemma (of_pair (to_pair x) = x) [SMTPat (to_pair x)]
 val lemma_to_of_inv (x: mant_pow) : Lemma (to_pair (of_pair x) = x) [SMTPat (of_pair x)]
 
-let zero : float = of_pair (0, 0)
+val zero : (z: float{z = of_pair (0, 0)})
+val one : (o: float{o = of_pair (1, 0)})
+
+type not_zero = (nz: float{nz <> zero})
 
 let mantissa (x: float) : GTot mantType = (to_pair x)._1
 let power (x: float) : GTot powerType = (to_pair x)._2
 
 
+let rec pow10 (x: nat) : GTot pos =
+  match x with
+  | 0 -> 1
+  | _ -> 10 * pow10 (x - 1)
 let rec incr_power (mp: mant_pow') : GTot (x: mant_pow'{x._1 % 10 = 0 ==> x._2 = 0}) (decreases (-mp._2)) =
     if mp._1 % 10 = 0 && mp._2 < 0
     then incr_power (mp._1 / 10, mp._2 + 1)
@@ -41,11 +49,6 @@ let norm_pair (mant_pow: mant_pow') : GTot (x: mant_pow'{x._1 % 10 = 0 ==> x._2 
   | 0 -> 0, 0
   | _ -> incr_power mant_pow
 
-  
-let rec pow10 (x: nat) : GTot pos =
-  match x with
-  | 0 -> 1
-  | _ -> 10 * pow10 (x - 1)
 
 val add (a b: float) : Pure float
   (requires True)
@@ -67,15 +70,88 @@ val sub (a b: float) : Pure float
     let b' = (mantissa b) * pow10 (pow_b - pow_min) in
     to_pair c = (a' - b', pow_min))
 
+val neg (a: float) : Pure float
+  (requires True)
+  (ensures fun b -> mantissa a = -(mantissa b) /\ power a = power b)
+
 val mul (a b: float) : Pure float
   (requires True)
   (ensures fun c -> to_pair c = norm_pair (mantissa a * mantissa b, power a + power b))
 
-// val div (a b: float) : Pure float
-//   (requires True)
-//   (ensures fun c -> )
+val div (a: float) (b: not_zero) : float
 
 val gt (a b: float) : Pure bool (requires True) (ensures fun c -> c <==> mantissa (a `sub` b) > 0)
 val lt (a b: float) : Pure bool (requires True) (ensures fun c -> c <==> mantissa (a `sub` b) < 0)
 val gte (a b: float) : Pure bool (requires True) (ensures fun c -> c <==> mantissa (a `sub` b) >= 0)
 val lte (a b: float) : Pure bool (requires True) (ensures fun c -> c <==> mantissa (a `sub` b) <= 0)
+
+unfold let ( +. ) a b = add a b
+unfold let ( -. ) a b = sub a b
+unfold let ( ~. ) a   = neg a
+unfold let ( *. ) a b = mul a b
+unfold let ( /. ) a b = div a b
+
+unfold let (>.) a b = gt a b
+unfold let (<.) a b = lt a b
+unfold let (>=.) a b = gte a b
+unfold let (<=.) a b = lte a b
+
+
+val abs (a: float) : Pure float
+  (requires True)
+  (ensures fun b -> (if a <. zero then b = ~.a else b = a) /\ b >=. zero)
+
+let lemma_commut_add a b : Lemma (a +. b = b +. a) = ()
+let lemma_commut_mul a b : Lemma (a *. b = b *. a) = ()
+
+let lemma_add_zero a : Lemma (a +. zero = a) = ()
+let lemma_mul_one  a : Lemma (a *. one  = a) = ()
+let lemma_mul_zero a : Lemma (a *. zero = zero) = ()
+
+let lemma_sub_neg a : Lemma (~.a = zero -. a) = ()
+let lemma_neg_neg a : Lemma (~.(~.a) = a) = ()
+let lemma_add_neg a : Lemma (a -. a = zero) = ()
+
+let lemma_additive_add_left a b c : Lemma (a +. b +. c = (a +. b) +. c) = ()
+let lemma_additive_add_right a b c : Lemma (a +. b +. c = a +. (b +. c)) [SMTPat (a +. b +. c)] =
+  assume (a +. b +. c = a +. (b +. c))
+let lemma_additive_mul_left a b c : Lemma (a *. b *. c = (a *. b) *. c) = ()
+let lemma_additive_mul_right a b c : Lemma (a *. b *. c = a *. (b *. c)) = 
+  assume (a *. b *. c = a *. (b *. c))
+
+let lemma_add_perenos a b c : Lemma (requires a +. b = c) (ensures a = c -. b) =
+  assert (a +. b -. b = c -. b);
+  lemma_additive_add_right a b (~.b)
+
+let lemma_distrib_add a b c : Lemma (a *. (b +. c) = a *. b +. a *. c) = assume (a *. (b +. c) = a *. b +. a *. c)
+
+// let lemma_gt a b : Lemma (requires a >. b) (ensures a -. b >. zero) = ()
+
+
+let ( .[] ) x (min, max) = min <=. x && x <=. max
+let ( .() ) x (min, max) = min <. x && x <. max
+let ( <.|> ) x (min, max) = min <=. x && x <. max
+let ( <|.> ) x (min, max) = min <. x && x <=. max
+
+let pi : float = of_int 180
+let piHalf : float = of_int 90
+
+val sin : float -> (r: float{r.[~.one, one]})
+val cos : float -> (r: float{r.[~.one, one]})
+val arctg (x y: float) : (r: float{r.[~.pi, pi]})
+val hypot (x y: float) : (r: float{r *. r = x *. x +. y *. y /\ r >=. zero})
+
+val lemma_sin_odd  (a: float) : Lemma (sin a = ~.(sin ~.a))
+val lemma_cos_even (a: float) : Lemma (cos a = cos ~.a)
+val lemma_arctg_x_pos x y : Lemma (requires x >=. zero) (ensures (arctg x y).(~.piHalf, piHalf)) [SMTPat (arctg x y)]
+
+val lemma_sin_0 (a: float{a = zero}) : Lemma (sin a = zero)
+val lemma_cos_0 (a: float{a = zero}) : Lemma (cos a = one)
+let lemma_sin_cos_0 (a: float{a = zero}) : Lemma (sin a = zero /\ cos a = one) = lemma_sin_0 a; lemma_cos_0 a
+
+val lemma_sin_90 (a: float{a = of_int 90}) : Lemma (sin a = one)
+val lemma_cos_90 (a: float{a = of_int 90}) : Lemma (cos a = zero)
+let lemma_sin_cos_90 (a: float{a = of_int 90}) : Lemma (sin a = one /\ cos a = zero) = lemma_sin_90 a; lemma_cos_90 a
+
+val lemma_cos_add (a b: float) : Lemma (cos (a +. b) = cos a *. cos b -. sin a *. sin b)
+val lemma_sin_add (a b: float) : Lemma (sin (a +. b) = sin a *. cos b +. cos a *. sin b)
