Test.Coordinates.fst
@@ -1,0 +1,26 @@
+module Test.Coordinates
+
+open Test.Float
+
+type azType = (az: float{az <.|> (~.pi, pi)})
+type psk : eqtype =
+  {
+    az: (az: float{az <.|> (~.pi, pi)});
+    um: (um: float{um.(~.piHalf, piHalf)})
+  }
+type cart : eqtype = { x: float; y: float; z: float}
+
+let psk2cart (coord: psk) = 
+  let x = cos coord.az *. cos coord.um in
+  let y = sin coord.az *. cos coord.um in
+  let z = sin coord.um in
+  { x = x; y = y; z = z }
+
+let cart2psk (coord: cart) =
+  let az = arctg coord.x coord.y in
+  let um = arctg (hypot coord.x coord.y) coord.z in
+  let az' = if az = pi then ~.pi else az in
+  { az = az'; um = um }
+
+// let lemma_psk2cart (p: psk) : Lemma (cart2psk (psk2cart p) = p) [SMTPat (psk2cart p)] =
+//   ()
