Test.Program.fst
@@ -3,20 +3,18 @@ module Test.Program
 open FStar.IO
 open Test.Float
 
-let f x =
-  let rec g y = y + 1 in
-  g x
 
 #push-options "--warn_error -272"
 let main =
   let x = of_pair (2, -1) in
   let y = of_pair (4, 0) in
-  let z = x `sub` y in
-  let b = z `gt` zero in
+  let z = x -. one in
+  assert (zero >=. zero);
+  assert (x -. y = ~. y +. x);
 
   let msg = Printf.ext_sprintf float_extension
-    "%Xf * %Xf = %Xf %b\n"
-    x y z b in
+    "%Xf * %Xf = %Xf\n"
+    x y z in
   print_string msg
 
 #pop-options
